repr/Test.v
@@ -1,0 +1,101 @@
+From Coq Require Import PrimString.
+From MetaCoq.Template Require Import All.
+From Repr Require Import All Utils.
+
+Unset MetaCoq Strict Unquote Universe Mode.
+
+(* Instances *)
+
+Instance repr_bytestring : Repr bytestring.string := 
+{ repr_doc _ s := group $ bracket """" (str $ pstring_of_bytestring s) """" }.
+
+Instance repr_sort : Repr sort :=
+{ repr_doc _ _ := str "#sort" }.
+
+MetaCoq Run (derive_global cast_kind).
+MetaCoq Run (derive_global name).
+MetaCoq Run (derive_global modpath).
+
+(* Testing *)
+
+(* TODO : 
+   1. handle records (it cannot be a fixpoint). 
+   2. handle abbreviations of inductives (+ better error messages). *)
+
+Definition x : ident := "x"%bs.
+Eval compute in repr x.
+
+(*Inductive term : Type :=
+  |	tRel : nat -> term
+  | tVar : ident -> term
+  | tEvar : nat -> list term -> term
+  | tSort : sort -> term
+  | tCast : term -> cast_kind -> term -> term
+  | tProd : aname -> term -> term -> term
+  | tLambda : aname -> term -> term -> term
+  | tLetIn : aname -> term -> term -> term -> term
+  | tApp : term -> list term -> term
+  | tConst : kername -> Instance.t -> term
+  | tInd : inductive -> Instance.t -> term
+  | tConstruct : inductive -> nat -> Instance.t -> term
+  | tCase : case_info -> predicate term -> term -> list (branch term) -> term
+  | tProj : projection -> term -> term
+  | tFix : mfixpoint term -> nat -> term
+  | tCoFix : mfixpoint term -> nat -> term
+  | tInt : PrimInt63.int -> term
+  | tFloat : PrimFloat.float -> term
+  | tString : pstring -> term
+  | tArray : Level.t -> list term -> term -> term -> term.
+*)*)
+
+(*
+(** SCRATCH *)
+
+
+Instance repr_nat : Repr nat :=
+{ repr_doc _ n := str $ pstring_of_nat n }.
+
+Instance repr_list {A} `{Repr A} : Repr (list A) :=
+{
+  repr_doc _ l := 
+    let contents := flow_map (str ";" ^^ break 1) (repr_doc 0) l in
+    group $ bracket "[" contents "]"
+}.
+
+Monomorphic Inductive vec A : nat -> Type :=
+  | VNil : vec A 0
+  | VCons : forall n, A -> vec A n -> vec A (S n).
+
+Fixpoint repr_vec_test (A : Type) n (_ : Repr A) (prec : nat) (xs : vec A n) {struct xs} : doc unit :=
+  let inst A' n' RA' := Build_Repr _ (repr_vec_test A' n' RA') in
+  match xs with 
+  | VNil => repr_ctor prec "VNil" []
+  | VCons n x xs => repr_ctor prec "VCons" [repr_arg n; repr_arg x; repr_arg xs]
+  end.
+
+Monomorphic Inductive tree A : nat -> A -> Type :=
+  | Leaf : forall a : A, tree A 0 a 
+  | Node : forall a n m, A -> tree (list A) n [a] -> tree A m a -> tree A (n + m) a.
+Arguments Leaf {A}.
+Arguments Node {A}.
+  
+Definition repr_tree_test :=
+  fix f 
+    (A : Type) 
+    (n : nat) (a : A) 
+    (RA : Repr A) 
+    (prec : nat) (xs : tree A n a) {struct xs} : doc unit :=
+    let _ := fun (A' : Type) (n' : nat) (a' : A') (RA' : Repr A') => Build_Repr _ (f A' n' a' RA') in 
+    match xs with 
+    | Leaf a => repr_ctor prec "Leaf" [repr_arg a]
+    | Node a n m x l r => repr_ctor prec "Node" [repr_arg a ; repr_arg n; repr_arg m ; repr_arg x; repr_arg l; repr_arg r]
+    end.
+
+(*Definition repr_tree' {A} {RA : Repr A} : Repr (tree A) := Build_Repr _ (repr_tree A RA).
+Existing Instance repr_tree'.
+
+Instance : Repr bool := { repr_doc b := if b then str "true" else str "false" }.
+
+Eval compute in repr $ Node true (Node [true; false; true] Leaf Leaf) (Node false Leaf Leaf).*)
+
+(** END SCRATCH *)*)
